template-rocq/theories/LoopChecking/UnivLoopChecking.v
@@ -2,7 +2,7 @@
 (* This module provides an instantiation of the deciders for universe checking,
   i.e. for constraints on non-empty level expressions (l, k) where k ∈ 𝐍 *)
 
-From Stdlib Require Import ssreflect ssrbool.
+From Stdlib Require Import ssreflect ssrfun ssrbool.
 From Stdlib Require Import Program RelationClasses Morphisms.
 From Stdlib Require Import Orders OrderedTypeAlt OrderedTypeEx MSetList MSetInterface MSetAVL MSetFacts FMapInterface MSetProperties MSetDecide.
 From MetaRocq.Utils Require Import utils.
@@ -16,7 +16,6 @@ Import Universes.
 Module MoreLevel.
   Import Universes.
   Include Level.
-
   Definition to_string := string_of_level.
 End MoreLevel.
 
@@ -94,11 +93,8 @@ End LevelExprZSet.
 Module LevelExprZSetFacts := WFactsOn LevelExprZ LevelExprZSet.
 Module LevelExprZSetProp := MSetProperties.OrdProperties LevelExprZSet.
 
-Module LevelSet.
-  Include MakeWithLeibniz Level.
-End LevelSet.
 Module LS <: LevelSets.
-  Module Level := MoreLevel .
+  Module Level := MoreLevel.
   Module LevelSet := LevelSet.
   Module LevelExpr := LevelExprZ.
   Module LevelExprSet := LevelExprZSet.
@@ -190,7 +186,6 @@ Next Obligation.
   congruence.
 Qed.
 
-
 Module UnivLoopChecking.
   Module LoopCheck := LoopChecking LS.
 
@@ -219,8 +214,11 @@ Module UnivLoopChecking.
   Record univ_model := {
     model : LoopCheck.model;
     constraints : UnivConstraintSet.t;
-    repr_constraints : forall c, UnivConstraintSet.In c constraints <->
-      Clauses.Subset (LoopCheck.to_clauses (to_constraint c)) (LoopCheck.Impl.Abstract.clauses model) }.
+    repr_constraints : forall c, UnivConstraintSet.In c constraints ->
+      Clauses.Subset (LoopCheck.to_clauses (to_constraint c)) (LoopCheck.Impl.Abstract.clauses model);
+    repr_constraints_inv : forall cl, Clauses.In cl (LoopCheck.Impl.Abstract.clauses model) ->
+      exists c, UnivConstraintSet.In c constraints /\ Clauses.In cl (LoopCheck.to_clauses (to_constraint c))
+      }.
 
   Module C := LoopCheck.Impl.I.Model.Model.Clauses.
   Import C.
@@ -235,6 +233,59 @@ Module UnivLoopChecking.
     rewrite Z2Nat.id //.
   Qed.
 
+  Lemma in_to_atoms a u :
+    LevelExprSet.In (a.1, Z.of_nat a.2) (to_atoms u) <-> Universes.LevelExprSet.In a u.
+  Proof.
+    destruct a as [l k].
+    rewrite /to_atoms //=.
+    split.
+    - move/to_levelexprzset_spec_2 => [] hin _.
+      now rewrite Nat2Z.id in hin.
+    - now move/to_levelexprzset_spec_1.
+  Qed.
+
+  Lemma univ_levels_spec l u :
+    Universes.LevelSet.In l (Universes.LevelExprSet.levels u) <->
+    exists k, Universes.LevelExprSet.In (l, k) u.
+  Proof.
+    rewrite /Universes.LevelExprSet.levels.
+    eapply Universes.LevelExprSetProp.fold_rec.
+    - move=> s' he; split. lsets.
+      move=> [k hin]. firstorder.
+    - move=> x a s' s'' hin hnin hadd.
+      rewrite Universes.LevelSet.add_spec.
+      split.
+      rewrite H. firstorder.
+      subst l. exists x.2. apply hadd. left. now destruct x.
+      intros [k' hin']. apply hadd in hin' as []; subst.
+      now left. now right; firstorder.
+  Qed.
+
+  Lemma levels_in_to_atoms l u :
+    LevelSet.In l (levels (to_atoms u)) <-> Universes.LevelSet.In l (Universes.LevelExprSet.levels u).
+  Proof.
+    rewrite levelexprset_levels_spec.
+    rewrite /in_to_atoms.
+    split.
+    - move=> [] k. move/to_levelexprzset_spec_2 => [] hin _.
+      apply univ_levels_spec. now eexists.
+    - rewrite univ_levels_spec => -[] k hin.
+      exists (Z.of_nat k). now rewrite (in_to_atoms (l, k)).
+  Qed.
+
+  Definition to_atom '(l, k) : LevelExpr.t := (l, Z.of_nat k).
+
+  Lemma exists_to_atoms_spec f u :
+    LevelExprSet.Exists f (to_atoms u) <->
+    exists le, Universes.LevelExprSet.In le u /\ f (to_atom le).
+  Proof.
+    rewrite /to_atoms //=; split; rewrite /LevelExprSet.Exists.
+    - move=> [] [] l k [] /to_levelexprzset_spec_2 [] hin hpos hf.
+      eexists; split; tea. cbn. rewrite Z2Nat.id //.
+    - move=> [] [] l k [] hin hf. exists (l, Z.of_nat k); split => //.
+      now apply to_levelexprzset_spec_1.
+    Qed.
+
   Lemma exists_to_atoms_2 a (u : Universe.t) :
     Universes.LevelExprSet.Exists (fun lk => a = lk) u ->
     LevelExprSet.Exists (fun lk : LevelExprSet.elt => a = (lk.1, Z.to_nat lk.2)) (to_atoms u).
@@ -245,38 +296,283 @@ Module UnivLoopChecking.
     rewrite Nat2Z.id //.
   Qed.
 
+  Definition choose (u : Universe.t) : Universes.LevelExpr.t := (Universes.NonEmptySetFacts.to_nonempty_list u).1.
+  Lemma choose_spec u : Universes.LevelExprSet.In (choose u) u.
+  Proof.
+    rewrite /choose.
+    have hs := Universes.NonEmptySetFacts.to_nonempty_list_spec u.
+    destruct Universes.NonEmptySetFacts.to_nonempty_list. cbn.
+    rewrite -Universes.LevelExprSet.elements_spec1 InA_In_eq -hs.
+    now constructor.
+  Qed.
+
+  Definition choose_prems (u : premises) : LevelExpr.t := (NonEmptySetFacts.to_nonempty_list u).1.
+  Lemma choose_prems_spec u : LevelExprSet.In (choose_prems u) u.
+  Proof.
+    rewrite /choose_prems.
+    have hs := NonEmptySetFacts.to_nonempty_list_spec u.
+    destruct NonEmptySetFacts.to_nonempty_list. cbn.
+    rewrite -LevelExprSet.elements_spec1 InA_In_eq -hs.
+    now constructor.
+  Qed.
+
+  Lemma clauses_of_le_nempty l r : ~ Clauses.Empty (LoopCheck.clauses_of_le l r).
+  Proof.
+    intros he. red in he. eapply he.
+    rewrite !LoopCheck.clauses_of_le_spec.
+    exists (choose_prems l). split; trea.
+    apply choose_prems_spec.
+  Qed.
+
+  Lemma to_clauses_ne c : ~ Clauses.Empty (LoopCheck.to_clauses c).
+  Proof.
+    intros he. red in he. destruct c as [[l []] r].
+    eapply he. apply LoopCheck.to_clauses_spec.
+    right. exists (choose_prems r). split; trea. apply choose_prems_spec.
+    eapply he. apply LoopCheck.to_clauses_spec.
+    exists (choose_prems l). split; trea. apply choose_prems_spec.
+  Qed.
+
+
   Equations? init_model : univ_model :=
   init_model := {| model := LoopCheck.init_model;
                    constraints := UnivConstraintSet.empty |}.
-  Proof. split; try ucsets.
-    move=> hyp; apply UnivConstraintSetFact.empty_iff.
-    destruct c as [[l d] r]. destruct d; cbn in hyp.
-    destruct Z.ltb. cbn in hyp.
-    move: hyp. rewrite /Clauses.Subset.
-    rw LoopCheck.clauses_of_le_spec.
-    move=> h.
-    have h' := fun a e => h _ (exists_to_atoms_2 _ _ e).
-    specialize (hyp ()) apply hyp.
-    2:{ }
-    de
-clset.
+  Proof.
+    move: H. now rewrite UnivConstraintSetFact.empty_iff.
+    move: H. now rewrite ClausesFact.empty_iff.
+  Qed.
+
+  Local Obligation Tactic := idtac.
+
+  Local Definition declare_levels_aux m l :=
+    LevelSet.fold (fun l m => match LoopCheck.declare_level m l return _ with None => m | Some m => m end) l m.
+
+  Lemma declare_levels_aux_spec m l : LoopCheck.levels (declare_levels_aux m l) =_lset
+    LevelSet.union l (LoopCheck.levels m).
+  Proof.
+    rewrite /declare_levels_aux.
+    eapply LevelSetProp.fold_rec.
+    - move=> s' he. lsets.
+    - move=> x a s' s'' hin hnin hadd heq.
+      apply LevelSetProp.Add_Equal in hadd.
+      destruct LoopCheck.declare_level eqn:decl.
+      * apply LoopCheck.declare_level_levels in decl as [hnin' ->].
+        rewrite hadd heq. lsets.
+      * apply LoopCheck.declare_level_None in decl.
+        rewrite heq hadd.
+        rewrite heq LevelSet.union_spec in decl.
+        destruct decl => //. lsets.
+  Qed.
+
+  Lemma declare_levels_aux_clauses m l :
+    LoopCheck.clauses (declare_levels_aux m l) =_clset LoopCheck.clauses m.
+  Proof.
+    rewrite /declare_levels_aux.
+    eapply LevelSetProp.fold_rec.
+    - move=> s' he. clsets.
+    - move=> x a s' s'' hin hnin hadd heq.
+      apply LevelSetProp.Add_Equal in hadd.
+      destruct LoopCheck.declare_level eqn:hd => //.
+      rewrite -heq.
+      apply LoopCheck.declare_level_clauses in hd.
+      unfold LoopCheck.clauses.
+      now rewrite hd.
+  Qed.
 
   (* We ignore errors here, which can happen only if the levels are already declared *)
-  Definition declare_levels (m : univ_model) (l : LevelSet.t) :=
-    LevelSet.fold (fun l m => match LoopCheck.declare_level l m with None => m | Some m => m end) l m.
+  Program Definition declare_levels (m : univ_model) (l : LevelSet.t) :=
+    {| model := declare_levels_aux m.(model) l; constraints := m.(constraints); |}.
+  Next Obligation.
+  Proof.
+    intros m l c.
+    rewrite [LoopCheck.Impl.Abstract.clauses _]declare_levels_aux_clauses => hin.
+    move: (repr_constraints m c hin) => h.
+    etransitivity; tea. reflexivity.
+  Qed.
+  Next Obligation.
+    move=> m l cl.
+    rewrite [LoopCheck.Impl.Abstract.clauses _]declare_levels_aux_clauses => hin.
+    now exact: repr_constraints_inv m cl hin.
+  Qed.
 
-  Definition enforce_level_constraints (m : univ_model) (l : ConstraintSet.t) :=
+  Equations? enforce m (c : UnivConstraint.t) : option _ :=
+    enforce m c with inspect (LoopCheck.enforce m.(model) (to_constraint c)) :=
+      | exist None eq => None
+      | exist (Some (inl m')) eq => Some (inl {| model := m'; constraints := UnivConstraintSet.add c m.(constraints) |})
+      | exist (Some (inr loop)) eq => Some (inr loop).
+  Proof.
+    - move=> c'.
+      move/LoopCheck.enforce_clauses: eq.
+      rewrite /LoopCheck.clauses => ->. rewrite UnivConstraintSet.add_spec => -[].
+      * move=> ->. clsets.
+      * move=> hin.
+        move: (repr_constraints m c' hin) => h. clsets.
+    - move/LoopCheck.enforce_clauses: eq.
+      rewrite /LoopCheck.clauses => -> c'.
+      rewrite UnivLoopChecking.Clauses.union_spec => -[].
+      * move/(repr_constraints_inv m c') => [] c2 [].
+        exists c2. split => //.
+        rewrite UnivConstraintSet.add_spec. now right.
+      * move=> hin. exists c. split => //.
+        rewrite UnivConstraintSet.add_spec. now left.
+  Qed.
+
+  Lemma in_clause_levels_of_le lev l r : LevelSet.In lev (clauses_levels (LoopCheck.clauses_of_le l r)) <->
+    LevelSet.In lev (levels l) \/ LevelSet.In lev (levels r).
+  Proof.
+    rewrite clauses_levels_spec.
+    setoid_rewrite LoopCheck.clauses_of_le_spec.
+    split.
+    - intros [cl [hex hin]].
+      apply clause_levels_spec in hin.
+      destruct hex as [le [inl ->]]. cbn in *. destruct hin; auto. subst.
+      left. now apply LoopCheck.Impl.in_levels.
+    - move=> [] hin.
+      * eapply levelexprset_levels_spec in hin as [k hin].
+        exists (r, (lev, k)). split => //. exists (lev, k). split => //.
+        apply clause_levels_spec. now right.
+      * eapply levelexprset_levels_spec in hin as [k hin].
+        exists (r, choose_prems l). split => //. exists (choose_prems l). split => //.
+        apply choose_prems_spec.
+        apply clause_levels_spec. left.
+        apply levelexprset_levels_spec. now exists k.
+  Qed.
+
+  Lemma univ_in_add n u : Universes.LevelSet.Equal
+    (Universes.LevelExprSet.levels (Universe.add n u))
+    (Universes.LevelExprSet.levels u).
+  Proof.
+    intros l. rewrite !univ_levels_spec.
+    rewrite /Universe.add. rw Universes.NonEmptySetFacts.map_spec.
+    firstorder. destruct x0; noconf H0; cbn. now exists n0.
+    exists (n + x), (l, x). split => //.
+  Qed.
+
+  Lemma clauses_levels_union cls cls' : clauses_levels (Clauses.union cls cls') =_lset
+    LevelSet.union (clauses_levels cls) (clauses_levels cls').
+  Proof.
+    intros l.
+    rewrite clauses_levels_spec LevelSet.union_spec.
+    rw Clauses.union_spec; rewrite !clauses_levels_spec.
+    rw clause_levels_spec. firstorder.
+  Qed.
+
+  Definition univ_constraint_levels (c : UnivConstraint.t) :=
+    let '(l, d, r) := c in
+    LevelSet.union (Universes.LevelExprSet.levels l)
+      (Universes.LevelExprSet.levels r).
+
+  Lemma declared_univ_cstr_levels_spec ls c :
+    declared_univ_cstr_levels ls c <->
+    univ_constraint_levels c ⊂_lset ls.
+  Proof.
+    destruct c as [[l d] r].
+    rewrite /declared_univ_cstr_levels /univ_constraint_levels.
+    split.
+    - move=> [] hl hr l'.
+      rewrite LevelSet.union_spec. firstorder.
+    - intros he; split => l'. specialize (he l').
+      rewrite LevelSet.union_spec in he. firstorder.
+      specialize(he l'). rewrite LevelSet.union_spec in he. firstorder.
+  Qed.
+
+  Definition constraint_levels (c : LoopCheck.constraint) :=
+    LevelSet.union (levels c.1.1) (levels c.2).
+
+  Lemma in_constraint_levels_to_constraint c :
+    forall l, LevelSet.In l (constraint_levels (to_constraint c)) <->
+      LevelSet.In l (univ_constraint_levels c).
+  Proof.
+    intros l; destruct c as [[l' d] r]; cbn.
+    rewrite /constraint_levels. rewrite !LevelSet.union_spec. cbn.
+    destruct d.
+    destruct Z.ltb.
+    - rewrite !levels_in_to_atoms. rewrite univ_in_add. firstorder.
+    - rewrite !levels_in_to_atoms. rewrite univ_in_add. firstorder.
+    - rewrite !levels_in_to_atoms. firstorder.
+  Qed.
+
+  Lemma in_to_clauses_levels c :
+    forall l, LevelSet.In l (clauses_levels (LoopCheck.to_clauses c)) <->
+      LevelSet.In l (constraint_levels c).
+  Proof.
+    intros l.
+    destruct c as [[l' d] r] => //=.
+    destruct d. rewrite clauses_levels_union LevelSet.union_spec.
+    rewrite /constraint_levels //= LevelSet.union_spec.
+    rewrite !in_clause_levels_of_le. firstorder.
+    rewrite /constraint_levels //= LevelSet.union_spec.
+    rewrite !in_clause_levels_of_le. firstorder.
+  Qed.
+
+  Lemma ndecl_nin_levels ls c :
+    declared_univ_cstr_levels ls c <->
+    clauses_levels (LoopCheck.to_clauses (to_constraint c)) ⊂_lset ls.
+  Proof.
+    rewrite declared_univ_cstr_levels_spec.
+    split; intros h.
+    - intros ?; rewrite in_to_clauses_levels in_constraint_levels_to_constraint. apply h.
+    - etransitivity; tea. intros ?.
+      now rewrite in_to_clauses_levels in_constraint_levels_to_constraint.
+  Qed.
+
+  Lemma enforce_not_none m c : enforce m c <> None <->
+    declared_univ_cstr_levels (LoopCheck.levels (model m)) c.
+  Proof.
+    have := @LoopCheck.enforce_not_None (model m) (to_constraint c).
+    rewrite /enforce.
+    destruct inspect as [[[] | ] eq]. simpl.
+    - intros. split => // _.
+      rewrite ndecl_nin_levels. apply H. now rewrite eq.
+    - intros. split => // _.
+      rewrite ndecl_nin_levels. apply H. now rewrite eq.
+    - intros. split => //=.
+      now move/ndecl_nin_levels/H; rewrite eq.
+  Qed.
+
+  Lemma enforce_None m c :
+    enforce m c = None <-> ~ declared_univ_cstr_levels (LoopCheck.levels m.(model)) c.
+  Proof.
+    rewrite /enforce.
+    destruct inspect as [[[] | ] eq]. simpl.
+    - intros. split => //.
+      rewrite ndecl_nin_levels.
+      rewrite -LoopCheck.enforce_not_None eq; elim. congruence.
+    - intros. split => //=.
+      rewrite ndecl_nin_levels.
+      rewrite -LoopCheck.enforce_not_None eq; elim. congruence.
+    - cbn. rewrite ndecl_nin_levels.
+      rewrite -LoopCheck.enforce_not_None eq. split => //. congruence.
+  Qed.
+
+  Definition levels m := LoopCheck.levels m.(model).
+
+  Lemma enforce_model m c m' :
+    enforce m c = Some (inl m') -> levels m = levels m' /\
+      UnivConstraintSet.Equal (UnivConstraintSet.add c (constraints m)) (constraints m').
+  Proof.
+    funelim (enforce m c) => //=.
+    move=> [=] <-; cbn. rewrite /levels //=.
+    split.
+    - clear H Heqcall. now move/LoopCheck.enforce_levels: eq.
+    - clear H Heqcall. reflexivity.
+  Qed.
+
+  Lemma model_satisfies m :
+    exists V, satisfies
+
+  (* Definition enforce_level_constraints (m : univ_model) (l : ConstraintSet.t) :=
     ConstraintSet.fold (fun c m =>
       match m with
       | inl m =>
         let c := (level_constraint_to_constraint c) in
-        match LoopCheck.enforce c m with
+        match LoopCheck.enforce m c with
         | None => (inr (c, None))
         | Some (inl m) => (inl m)
         | Some (inr u) => (inr (c, Some u))
         end
       | inr err => inr err
-      end) l (inl m).
+      end) l (inl m). *)
 
   Import LoopCheck.Impl.I.Model.Model.Clauses.FLS.
 
@@ -288,13 +584,5 @@ clset.
       end
     in
     (from_atoms l, d', from_atoms r).
-
-  Definition enforce (c : UnivConstraint.t) (m : univ_model) :=
-    match LoopCheck.enforce (to_constraint c) m with
-    |
-
-
-
-
 
 End UnivLoopChecking.
