common/theories/LoopChecking/Common.v
@@ -17,6 +17,8 @@ Notation fwd := (ltac:(move=> /(_ _)/Wrap[])).
 Arguments exist {A P}.
 Definition inspect {A} (x : A) : { y : A | x = y } := exist x eq_refl.
 
+Arguments symmetry {A R Symmetric} {x y}.
+
 #[program] Global Instance reflect_eq_Z : ReflectEq Z := {
     eqb := Z.eqb
   }.
